Makefile
@@ -20,7 +20,18 @@ proof: Makefile.coq $(COQTHEORIES)
 	$(MAKE) -f Makefile.coq $(patsubst %.v,%.vo,$(COQTHEORIES))
 
 Makefile.coq: Makefile $(COQTHEORIES)
-	(echo "-R lib $(COQMODULE)"; \
+	(echo "-R ../CompCert-intptr/lib compcertip.lib"; \
+	echo "-R ../CompCert-intptr/common compcertip.common"; \
+	echo "-R ../CompCert-intptr/x86 compcertip.x86"; \
+	echo "-R ../CompCert-intptr/x86_64 compcertip.x86_64"; \
+	echo "-R ../CompCert-intptr/backend compcertip.backend"; \
+	echo "-R ../CompCert-intptr/cfrontend compcertip.cfrontend"; \
+	echo "-R ../CompCert-intptr/driver compcertip.driver"; \
+	echo "-R ../CompCert-intptr/exportclight compcertip.exportclight"; \
+	echo "-R ../CompCert-intptr/flocq Flocq"; \
+	echo "-R ../CompCert-intptr/cparser compcertip.cparser"; \
+                          \
+		 echo "-R lib $(COQMODULE)"; \
          echo "-R ems $(COQMODULE)"; \
          echo "-R spc $(COQMODULE)"; \
          echo "-R proofmode $(COQMODULE)"; \
